@prefix rdf: <http://www.w3.org/1999/02/22-rdf-syntax-ns#>.
@prefix rdfs: <http://www.w3.org/2000/01/rdf-schema#>.
@prefix xsd: <http://www.w3.org/2001/XMLSchema#>.
@prefix dc: <http://purl.org/dc/elements/1.1/>.
@prefix dcterms: <http://purl.org/dc/terms/>.
@prefix dcmitype: <http://purl.org/dc/terms/DCMIType> .
@prefix dcat: <http://www.w3.org/ns/dcat#>.
@prefix skos: <http://www.w3.org/2004/02/skos/core#>.
@prefix qb: <http://purl.org/linked-data/cube#>.
@prefix owl: <http://www.w3.org/2002/07/owl#>.
@prefix disco: <http://rdf-vocabulary.ddialliance.org/discovery#>.
@prefix foaf: <http://xmlns.com/foaf/0.1/>.
@prefix adms: <http://www.w3.org/ns/adms#>.
@prefix org: <http://www.w3.org/ns/org#>.
@prefix prov: <http://www.w3.org/ns/prov#>.
@prefix xkos: <http://purl.org/linked-data/xkos#>.
@prefix sfi: <https://dhhepting.github.io/sfi#>.

sfi:FrequencyRepr a skos:ConceptScheme, disco:Representation;
	skos:hasTopConcept sfi:FNever, sfi:FRarely, sfi:FSometimes, sfi:FOften, sfi:FAlways .

sfi:FNever a skos:Concept;
	skos:notation "1"^^xsd:integer;
	skos:prefLabel "Never";
	skos:inScheme sfi:FrequencyRepr.

sfi:FRarely a skos:Concept;
	skos:notation "2"^^xsd:integer;
	skos:prefLabel "Rarely";
	skos:inScheme sfi:FrequencyRepr.

sfi:FSometimes a skos:Concept;
	skos:notation "3"^^xsd:integer;
	skos:prefLabel "Sometimes";
	skos:inScheme sfi:FrequencyRepr.

sfi:FOften a skos:Concept;
	skos:notation "4"^^xsd:integer;
 	skos:prefLabel "Often";
 	skos:inScheme sfi:FrequencyRepr.

sfi:FAlways a skos:Concept;
 	skos:notation "5"^^xsd:integer;
 	skos:prefLabel "Always";
 	skos:inScheme sfi:FrequencyRepr.

sfi:sfi_1 a disco:Questionnaire;
	disco:question sfi:FreqRating1WellPrepared;
	disco:question sfi:FreqRating2ClearExpectationsPrepPart;
	disco:question sfi:FreqRating3UsesTimeEffectively;
	disco:question sfi:FreqRating4ClearExpectationsAssignments;
	disco:question sfi:FreqRating5EncouragesParticipation;
	disco:question sfi:FreqRating6ClearlyAnswersQuestions;
	disco:question sfi:FreqRating7RespectsStudents;
	disco:question sfi:FreqRating8StimulatesDiscussions;
	disco:question sfi:FreqRating9EncouragesStudentQA;
 
	disco:question sfi:OpenEnded1CourseLikeBest;
	disco:question sfi:OpenEnded2CourseLikeToChange; 
	disco:question sfi:OpenEnded3InstructorStrengths.

sfi:FreqRating1WellPrepared a disco:Question;
	disco:questionText "1. The instructor is well-prepared for class."@en;
	disco:responseDomain sfi:FrequencyRepr.

sfi:FreqRating2ClearExpectationsPrepPart a disco:Question;
	disco:questionText "2. The instructor clearly communicates his expectations for student preparation and participation."@en;
	disco:responseDomain sfi:FrequencyRepr.

sfi:FreqRating3UsesTimeEffectively a disco:Question;
	disco:questionText "3. The instructor uses class time effectively."@en;
	disco:responseDomain sfi:FrequencyRepr.

sfi:FreqRating4ClearExpectationsAssignments a disco:Question;
	disco:questionText "4. The instructor has clear expectations for assigned work."@en;
	disco:responseDomain sfi:FrequencyRepr.

sfi:FreqRating5EncouragesParticipation a disco:Question;
	disco:questionText "5. The instructor encourages student participation."@en;
	disco:responseDomain sfi:FrequencyRepr.

sfi:FreqRating6ClearlyAnswersQuestions a disco:Question;
	disco:questionText "6. The instructor clearly answers questions."@en;
	disco:responseDomain sfi:FrequencyRepr.

sfi:FreqRating7RespectsStudents a disco:Question;
	disco:questionText "7. The instructor treats students with respect."@en;
	disco:responseDomain sfi:FrequencyRepr.

sfi:FreqRating8StimulatesDiscussions a disco:Question;
	disco:questionText "8. The instructor effectively directs and stimulates discussion."@en;
	disco:responseDomain sfi:FrequencyRepr.

sfi:FreqRating9EncouragesStudentQA a disco:Question;
	disco:questionText "9. The instructor effectively encourages students to ask questions and give answers."@en;
	disco:responseDomain sfi:FrequencyRepr.

sfi:OpenEnded1CourseLikeBest a disco:Question;
	disco:questionText "1. What do you like best about this course?"@en;
 	disco:responseDomain xsd:string.

sfi:OpenEnded2CourseLikeToChange a disco:Question;
	disco:questionText "2. What would you like to change about this course?"@en;
	disco:responseDomain xsd:string.

sfi:OpenEnded3InstructorStrengths a disco:Question;
	disco:questionText "3. What do you think are the instructor's greatest strengths?"@en;
 	disco:responseDomain xsd:string.

### Variables

sfi:FrequencyVD a disco:RepresentedVariable;
   disco:representation sfi:FrequencyRepr;
   skos:prefLabel "Frequency (Never - Always)"@en;
   dcterms:description "5-point Likert Scale for frequency (Never, Rarely, Sometimes, Often, Always)"@en.

sfi:FR1wellPrepared a disco:Variable;
   dcterms:identifier "FR1wellPrepared";
   skos:prefLabel "Instructor well-prepared"@en;
   dcterms:description "Frequency rating for the instructor being well-prepared."@en;
   disco:basedOn sfi:FreqencyVD;
   disco:question sfi:FreqRating1WellPrepared.

sfi:FR2clearExpPrepPart a disco:Variable;
   dcterms:identifier "FR2clearExpPrepPart";
   skos:prefLabel "Instructor clearly communicates expectations for student preparation and participation"@en;
   dcterms:description "Frequency rating for the instructor clearly communicating expectations for student preparation and participation. "@en;
   disco:basedOn sfi:FreqencyVD;
   disco:question sfi:FreqRating2ClearExpectationsPrepPart.

sfi:FR3usesTimeEffectively a disco:Variable;
   dcterms:identifier "FR3usesTimeEffectively";
   skos:prefLabel "Instructor uses time effectively"@en;
   dcterms:description "The frequency rating for the instructor using time effectively."@en;
   disco:basedOn sfi:FreqencyVD;
   disco:question sfi:FreqRating3UsesTimeEffectively.

sfi:FR4clearExpAssigned a disco:Variable;
   dcterms:identifier "FR4clearExpAssigned";
   skos:prefLabel "Instructor clearly communicates expectations of assigned work"@en;
   dcterms:description "Frequency rating for the instructor clearly communicating expectations for assigned work."@en;
   disco:basedOn sfi:FreqencyVD;
   disco:question sfi:FreqRating4ClearExpectationsAssignments.

sfi:FR5encouragesPart a disco:Variable;
   dcterms:identifier "FR5encouragesPart";
   skos:prefLabel "Instructor encourages student participation"@en;
   dcterms:description "The frequency rating for the instructor encouraging student participation."@en;
   disco:basedOn sfi:FreqencyVD;
   disco:question sfi:FreqRating5EncouragesParticipation.

sfi:FR6clearlyAnswersQs a disco:Variable;
   dcterms:identifier "FR6clearlyAnswersQs";
   skos:prefLabel "Instructor clearly answers questions"@en;
   dcterms:description "The frequency rating for the instructor clearly answering questions."@en;
   disco:basedOn sfi:FreqencyVD;
   disco:question sfi:FreqRating6ClearlyAnswersQuestions.

sfi:FR7respectsStudents a disco:Variable;
   dcterms:identifier "FR7respectsStudents";
   skos:prefLabel "Instructor respects students"@en;
   dcterms:description "The frequency rating for the instructor respecting students."@en;
   disco:basedOn sfi:FreqencyVD;
   disco:question sfi:FreqRating7RespectsStudents.

sfi:FR8stimulatesDiscuss a disco:Variable;
   dcterms:identifier "FR8stimulatesDiscuss";
   skos:prefLabel "Instructor stimulates discussions"@en;
   dcterms:description "The frequency rating for the instructor stimulating discussions."@en;
   disco:basedOn sfi:FreqencyVD;
   disco:question sfi:FreqRating8StimulatesDiscussions.

sfi:FR9encouragesQA a disco:Variable;
   dcterms:identifier "FR9encouragesQA";
   skos:prefLabel "Instructor encourages questions and answers"@en;
   dcterms:description "The frequency rating for the instructor encouraging questions and answers."@en;
   disco:basedOn sfi:FreqencyVD;
   disco:question sfi:FreqRating9EncouragesStudentQA.

sfi:OpenEndedTextRespVD a disco:RepresentedVariable;
   disco:representation xsd:string;
   skos:prefLabel "Open Ended Textual Response"@en;
   dcterms:description "Open Ended Textual Response."@en.

sfi:OE1courseLikeBest a disco:Variable;
	dcterms:identifier "OE1courseLikeBest";
	skos:prefLabel "Liked Best about Course"@en;
	dcterms:description "A textual response about what is liked best about the course."@en;
	disco:basedOn sfi:OpenEndedTextRespVD;
	disco:question sfi:OpenEnded1CourseLikeBest.

sfi:OE2courseLikeToChange a disco:Variable;
   dcterms:identifier "OE2courseLikeToChange";
   skos:prefLabel "Like to Change about Course"@en;
   dcterms:description "A textual response about what is liked best about the course."@en;
   disco:basedOn sfi:OpenEndedTextRespVD;
   disco:question sfi:OpenEnded2CourseLikeToChange. 

sfi:OE3instructorStrengths a disco:Variable;
   dcterms:identifier "OE3instructorStrengths";
   skos:prefLabel "Instructor Strengths"@en;
   dcterms:description "A textual response about the instructorâ€™s greatest strengths."@en;
   disco:basedOn sfi:OpenEndedTextRespVD;
   disco:question sfi:OpenEnded3InstructorStrengths.
